Etch/StreamFusion/Benchmark-CountEmployeesOfSmallCompanies.lean
@@ -20,17 +20,15 @@ abbrev CSTATE := String -- State the company is employed in
 
 @[inline]
 def countEmplyeesOfSmallCompanies
-    [ToStream E (EID →ₛ ENAME →ₛ CID →ₛ Bool)]
-    [ToStream C (CID →ₛ CNAME →ₛ ENUM →ₛ CSTATE →ₛ ℕ)]
-    (employeeStream : E)
-    (companyStream : C)
+    (employee : (EID →ₛ ENAME →ₛ CID →ₛ Bool))
+    (company : (CID →ₛ CNAME →ₛ ENUM →ₛ CSTATE →ₛ ℕ))
     : EID →ₛ ENAME →ₛ Unit →ₛ CNAME →ₛ ENUM →ₛ CSTATE →ₛ ℕ :=
 
   let S := [(eid,EID),(ename,ENAME),(cid,CID),(cname,CNAME),(enum,ENUM),(cstate,CSTATE)]
-  let employees := { S | employeeStream(eid,ename,cid) }
-  let companies := { S | companyStream(cid,cname,enum,cstate) }
-  let inCal   := S ⇑ (idx (singleton "CA") [cstate])
-  let leFifty := S ⇑ (idx (SStream.le 50) [enum])
+  let employees :=  S ⇑ employee(eid,ename,cid)
+  let companies :=  S ⇑ company(cid,cname,enum,cstate)
+  let inCal   := S ⇑ (singleton "CA")(cstate)
+  let leFifty := S ⇑ (SStream.le 50)(enum)
   let result := Σ cid: inCal * leFifty * employees * companies
   result
 
